Bad attempt to fix the literals and move list lemmas to the right place

src/Init/Data/String/Bootstrap.lean
@@ -127,9 +127,30 @@ opaque dropRight (s : String) (n : Nat) : String
 
 end String.Internal
 
-@[extern "lean_string_mk", expose]
-def String.mk (s : List Char) : String :=
-  ⟨List.utf8Encode s, .intro s rfl⟩
+-- axiom String.mk (data : List Char) : String
+
+-- @[extern "lean_string_mk"]
+-- def String.mk (data : List Char) : String :=
+--   ⟨List.utf8Encode data,.intro data rfl⟩
+
+opaque String.opaqueFoo (data : List Char) : { s : String // s.bytes = List.utf8Encode data } :=
+  ⟨⟨List.utf8Encode data, .intro data rfl⟩, rfl⟩
+
+/--
+Creates a string that contains the characters in a list, in order.
+
+Examples:
+ * `['L', '∃', '∀', 'N'].asString = "L∃∀N"`
+ * `[].asString = ""`
+ * `['a', 'a', 'a'].asString = "aaa"`
+-/
+@[extern "lean_string_mk"]
+def String.mk (data : List Char) : String :=
+  String.opaqueFoo data
+
+@[simp]
+theorem String.bytes_mk {data : List Char} : (String.mk data).bytes = List.utf8Encode data :=
+  (String.opaqueFoo data).2
 
 /--
 Creates a string that contains the characters in a list, in order.
